[Civl] Generalize inductive sequentialization proof rule (#687)
* first commit

* removed pendingAsyncs variable

Test/civl/inductive-sequentialization/paxos/Paxos.bpl
@@ -111,7 +111,6 @@ function {:inline} VotePAs(r: Round, v: Value) : [PA]int
 // Abstract
 var {:layer 1,3} joinedNodes: [Round]NodeSet;
 var {:layer 1,3} voteInfo: [Round]Option VoteInfo;
-var {:layer 1,3} pendingAsyncs: [PA]int;
 
 // Concrete
 var {:layer 0,1} acceptorState: [Node]AcceptorState;
@@ -127,13 +126,12 @@ var {:layer 1,1} {:linear "perm"} permVoteChannel: VoteResponseChannel;
 
 function {:inline} Init (
   rs: [Round]bool, joinedNodes:[Round]NodeSet, voteInfo: [Round]Option VoteInfo,
-  decision:[Round]Option Value, pendingAsyncs: [PA]int) : bool
+  decision:[Round]Option Value) : bool
 {
   rs == (lambda r: Round :: true) &&
   (forall r: Round :: joinedNodes[r] == NoNodes()) &&
   (forall r: Round :: voteInfo[r] is None) &&
-  (forall r: Round :: decision[r] is None) &&
-  (forall pa: PA :: pendingAsyncs[pa] == 0)
+  (forall r: Round :: decision[r] is None)
 }
 
 function {:inline} InitLow (
