Test/civl/inductive-sequentialization/paxos/is.sh
@@ -1,6 +1,6 @@
 #!/bin/bash
 
-# RUN: %parallel-boogie Paxos.bpl PaxosActions.bpl PaxosAbstractions.bpl PaxosSeq.bpl > "%t"
+# RUN: %parallel-boogie Paxos.bpl PaxosActions.bpl PaxosSeq.bpl > "%t"
 # RUN: %diff "%s.expect" "%t"
 
-boogie $@ /lib:base Paxos.bpl PaxosActions.bpl PaxosAbstractions.bpl PaxosSeq.bpl
+boogie $@ Paxos.bpl PaxosActions.bpl PaxosSeq.bpl
